src/Crypto/AESEncryption.dfy
@@ -1,36 +1,44 @@
 include "../SDK/AlgorithmSuite.dfy"
 include "../StandardLibrary/StandardLibrary.dfy"
-include "EncryptionParameters.dfy"
+include "EncryptionAlgorithms.dfy"
 include "GenBytes.dfy"
 
 module {:extern "AESEncryption"} AESEncryption {
-  import EncryptionParameters
+  import EncryptionAlgorithms
   import opened StandardLibrary
   import opened UInt = StandardLibrary.UInt
 
   export
-    provides AESDecrypt, AESEncrypt, EncryptionParameters, StandardLibrary, UInt
-    reveals EncryptionArtifacts
+    provides AESDecrypt, AESEncrypt, EncryptionAlgorithms, StandardLibrary, UInt
+    reveals EncryptionOutput
 
   // Is there a better name/location for this?
-  datatype EncryptionArtifacts = EncryptionArtifacts(cipherText: seq<uint8>, authTag: seq<uint8>)
+  datatype EncryptionOutput = EncryptionOutput(cipherText: seq<uint8>, authTag: seq<uint8>)
 
-  function method EncryptionArtifactFromByteSeq(s: seq<uint8>, p: EncryptionParameters.Params): (encArt: EncryptionArtifacts)
+  function method EncryptionArtifactFromByteSeq(s: seq<uint8>, p: EncryptionAlgorithms.Params): (encArt: EncryptionOutput)
+    requires p.Valid()
     requires |s| >= p.tagLen as int
-    ensures |encArt.cipherText + encArt.authTag| <= |s|
+    ensures |encArt.cipherText + encArt.authTag| == |s|
     ensures |encArt.authTag| == p.tagLen as int
   {
-    EncryptionArtifacts(s[.. |s| - p.tagLen as int], s[|s| - p.tagLen as int ..])
+    EncryptionOutput(s[.. |s| - p.tagLen as int], s[|s| - p.tagLen as int ..])
   }
 
-  method {:extern "AESEncryption.AES_GCM", "AESEncrypt"} AESEncrypt(params: EncryptionParameters.Params, iv: seq<uint8>, key: seq<uint8>, msg: seq<uint8>, aad: seq<uint8>)
-      returns (res : Result<EncryptionArtifacts>)
+  method {:extern "AESEncryption.AES_GCM", "AESEncrypt"} AESEncrypt(params: EncryptionAlgorithms.Params, iv: seq<uint8>, key: seq<uint8>, msg: seq<uint8>, aad: seq<uint8>)
+      returns (res : Result<EncryptionOutput>)
+    requires params.Valid()
+    requires params.alg.AES?
+    requires params.mode.GCM?
     requires |iv| == params.ivLen as int
     requires |key| == params.keyLen as int
     ensures res.Success? ==> |res.value.authTag| == params.tagLen as int
 
-  method {:extern "AESEncryption.AES_GCM", "AESDecrypt"} AESDecrypt(params: EncryptionParameters.Params, key: seq<uint8>, cipherTxt: seq<uint8>, authTag: seq<uint8>, iv: seq<uint8>, aad: seq<uint8>)
+  method {:extern "AESEncryption.AES_GCM", "AESDecrypt"} AESDecrypt(params: EncryptionAlgorithms.Params, key: seq<uint8>, cipherTxt: seq<uint8>, authTag: seq<uint8>, iv: seq<uint8>, aad: seq<uint8>)
       returns (res: Result<seq<uint8>>)
+    requires params.Valid()
+    requires params.alg.AES?
+    requires params.mode.GCM?
     requires |key| == params.keyLen as int
+    requires |iv| == params.ivLen as int 
     requires |authTag| == params.tagLen as int
 }
